theories/ftlr/AddSubLt.v
@@ -1,10 +1,10 @@
 From cap_machine Require Export logrel.
 From cap_machine.rules Require Export rules_AddSubLt.
-From cap_machine.rules Require Import rules_base.
 From iris.proofmode Require Import tactics.
 From iris.program_logic Require Import weakestpre adequacy lifting.
 From stdpp Require Import base.
 From cap_machine Require Import machine_base.
+From cap_machine.rules Require Import rules_base.
 
 Section fundamental.
   Context {Σ:gFunctors} {memg:memG Σ} {regg:regG Σ}
