theories/logrel.v
@@ -4,6 +4,7 @@ From iris.program_logic Require Export weakestpre.
 From cap_machine Require Export cap_lang region.
 From iris.algebra Require Import gmap agree auth.
 From iris.base_logic Require Export invariants na_invariants saved_prop.
+From cap_machine.rules Require Import rules_base.
 Import uPred.
 
 Ltac auto_equiv :=
