theories/rules/rules_Jnz.v
@@ -1,8 +1,8 @@
-From cap_machine Require Import rules_base.
 From iris.base_logic Require Export invariants gen_heap.
 From iris.program_logic Require Export weakestpre ectx_lifting.
 From iris.proofmode Require Import tactics.
 From iris.algebra Require Import frac.
+From cap_machine Require Export rules_base.
 
 Section cap_lang_rules.
   Context `{memG Σ, regG Σ}.
